{
 "cells": [
  {
   "cell_type": "code",
   "execution_count": null,
   "id": "fb493331-4f85-438a-95b2-b43021969835",
   "metadata": {},
   "outputs": [],
   "source": [
    "#1. Find the value of T(2) for the recurrence relation T(n) = 3T(n-1) + 12n, given that T(0)=5.\n",
    "\"\"\"\n",
    "We can solve this recurrence relation by iteratively substituting the values of T(n-1), T(n-2), and so on, until we reach the base case T(0).\n",
    "\n",
    "Here's the breakdown:\n",
    "\n",
    "T(1):\n",
    "T(1) = 3T(0) + 121 = 35 + 12 = 27\n",
    "\n",
    "T(2):\n",
    "T(2) = 3T(1) + 122 = 327 + 24 = 105\n",
    "\n",
    "Therefore, T(2) = 105.\n",
    "\"\"\"\n"
   ]
  },
  {
   "cell_type": "code",
   "execution_count": null,
   "id": "fd99fd8d-a927-48ec-9faf-77fd752d6f53",
   "metadata": {},
   "outputs": [],
   "source": [
    "#2. Given a recurrence relation, solve it using the substitution method:\n",
    "\n",
    "#a. T(n) = T(n-1) + c\n",
    "\n",
    "#b. T(n) = 2T(n/2) + n\n",
    "\n",
    "#c. T(n) = 2T(n/2) + c\n",
    "\n",
    "#d. T(n) = T(n/2) + c\n",
    "\n",
    "\"\"\"\n",
    "a. T(n) = T(n-1) + c\n",
    "\n",
    "We can directly substitute T(n-1) with its equivalent expression and continue until we reach the base case.\n",
    "\n",
    "T(n) = T(n-1) + c\n",
    "= (T(n-2) + c) + c\n",
    "= T(n-2) + 2c\n",
    "= (T(n-3) + c) + 2c\n",
    "= T(n-3) + 3c\n",
    "...\n",
    "= T(n-k) + kc\n",
    "\n",
    "If we let n-k = 0, then k = n.\n",
    "\n",
    "Therefore, T(n) = T(0) + nc.\n",
    "\n",
    "b. T(n) = 2T(n/2) + n\n",
    "\n",
    "We'll substitute T(n/2) repeatedly, halving n each time:\n",
    "\n",
    "T(n) = 2T(n/2) + n\n",
    "= 2(2T(n/4) + n/2) + n\n",
    "= 4T(n/4) + 2n\n",
    "= 4(2T(n/8) + n/4) + 2n\n",
    "= 8T(n/8) + 3n\n",
    "...\n",
    "= 2^kT(n/2^k) + kn\n",
    "\n",
    "If we let n/2^k = 1, then k = log2(n).\n",
    "\n",
    "Therefore, T(n) = 2^log2(n)T(1) + nlog2(n) = nT(1) + nlog2(n).\n",
    "\n",
    "c. T(n) = 2T(n/2) + c\n",
    "\n",
    "Similar to the previous case, we substitute T(n/2) repeatedly:\n",
    "\n",
    "T(n) = 2T(n/2) + c\n",
    "= 2(2T(n/4) + c) + c\n",
    "= 4T(n/4) + 3c\n",
    "= 4(2T(n/8) + c) + 3c\n",
    "= 8T(n/8) + 7c\n",
    "...\n",
    "= 2^kT(n/2^k) + (2^k - 1)c\n",
    "\n",
    "Again, letting n/2^k = 1, we get k = log2(n).\n",
    "\n",
    "Therefore, T(n) = 2^log2(n)T(1) + (2^log2(n) - 1)c = nT(1) + (n - 1)c.\n",
    "\n",
    "d. T(n) = T(n/2) + c\n",
    "\n",
    "Substituting T(n/2) repeatedly:\n",
    "\n",
    "T(n) = T(n/2) + c\n",
    "= (T(n/4) + c) + c\n",
    "= T(n/4) + 2c\n",
    "= (T(n/8) + c) + 2c\n",
    "= T(n/8) + 3c\n",
    "...\n",
    "= T(n/2^k) + kc\n",
    "\n",
    "Letting n/2^k = 1, we get k = log2(n).\n",
    "\n",
    "Therefore, T(n) = T(1) + log2(n)c.\n",
    "\n",
    "By using the substitution method, we've derived the closed-form solutions for each recurrence relation.\n",
    "\"\"\""
   ]
  },
  {
   "cell_type": "code",
   "execution_count": null,
   "id": "73418d59-5f7c-4965-bee3-adff3da7c981",
   "metadata": {},
   "outputs": [],
   "source": [
    "#3. Given a recurrence relation, solve it using the recursive tree approach:\n",
    "\n",
    "#a. T(n) = 2T(n-1) +1\n",
    "\n",
    "#b. T(n) = 2T(n/2) + n\n",
    "\n",
    "\n",
    "\"\"\"\n",
    "a. T(n) = 2T(n-1) + 1\n",
    "\n",
    "To visualize the recursive tree, let's consider the first few levels of the tree:\n",
    "\n",
    "T(n)\n",
    "  / \\\n",
    "2T(n-1) 1\n",
    " / \\\n",
    "4T(n-2) 2\n",
    " / \\\n",
    "8T(n-3) 4\n",
    " ...\n",
    "Each level adds 2^i nodes, and the cost of each node at level i is 1. So, the total cost at level i is 2^i.\n",
    "\n",
    "The tree has a height of n.\n",
    "\n",
    "Therefore, the total cost of the tree is the sum of the costs at each level:\n",
    "\n",
    "T(n) = 1 + 2 + 4 + ... + 2^(n-1)\n",
    "\n",
    "This is a geometric series with a common ratio of 2. The sum of a geometric series is given by:\n",
    "\n",
    "S = a(r^n - 1) / (r - 1)\n",
    "\n",
    "In this case, a = 1, r = 2, and n = n.\n",
    "\n",
    "So, T(n) = (2^n - 1) / (2 - 1) = 2^n - 1.\n",
    "\n",
    "b. T(n) = 2T(n/2) + n\n",
    "\n",
    "The recursive tree for this recurrence relation looks like:\n",
    "\n",
    "T(n)\n",
    "  / \\\n",
    "2T(n/2) n\n",
    " / \\   |\n",
    "4T(n/4) n/2 n\n",
    " / \\   |   |\n",
    "8T(n/8) n/4 n/2 n\n",
    " ...\n",
    "The height of the tree is log2(n). At each level i, there are 2^i nodes, and the cost of each node at level i is n/(2^i).\n",
    "\n",
    "So, the total cost at level i is 2^i * (n/(2^i)) = n.\n",
    "\n",
    "Therefore, the total cost of the tree is the sum of the costs at each level:\n",
    "\n",
    "T(n) = n * log2(n)\n",
    "\n",
    "\"\"\""
   ]
  }
 ],
 "metadata": {
  "kernelspec": {
   "display_name": "Python 3 (ipykernel)",
   "language": "python",
   "name": "python3"
  },
  "language_info": {
   "codemirror_mode": {
    "name": "ipython",
    "version": 3
   },
   "file_extension": ".py",
   "mimetype": "text/x-python",
   "name": "python",
   "nbconvert_exporter": "python",
   "pygments_lexer": "ipython3",
   "version": "3.12.4"
  }
 },
 "nbformat": 4,
 "nbformat_minor": 5
}
